theories/Symbolic/Solver.v
@@ -411,6 +411,7 @@ Module Type GenericSolverOn
           | bop.bvor => simplify_eq_binop_default_val bop.bvor
           | bop.bvxor => simplify_eq_binop_default_val bop.bvxor
           | bop.coalesce => simplify_eq_binop_default_val bop.coalesce
+          | bop.mulx => simplify_eq_binop_default_val bop.mulx
           | bop.bvapp => simplify_eq_binop_bvapp_val
           | bop.bvcons => simplify_eq_binop_bvcons_val
           | bop.update_vector_subrange s l =>
@@ -727,6 +728,7 @@ Module Type GenericSolverOn
             (fun (*bvtake*) _ _ _ => default)
             (fun (*expand*) _ _ => default)
             (fun (*coalesce*) _ _ _ => default)
+            (fun (*mulx*) _ _ _ => default)
             t e.
 
         Definition simplify_eq_binop_bvapp {m n} (t1 : Term Σ (ty.bvec m))
@@ -773,6 +775,7 @@ Module Type GenericSolverOn
             (fun (*bvtake*) _ _ _ => default)
             (fun (*expand*) _ _ => default)
             (fun (*coalesce*) _ _ _ => default)
+            (fun (*mulx*) _ _ _ => default)
             t e.
 
         Definition simplify_eq_binop_bvcons {m} (t1 : Term Σ ty.bool)
@@ -826,6 +829,7 @@ Module Type GenericSolverOn
           | bop.bvor => simplify_eq_binop_default bop.bvor
           | bop.bvxor => simplify_eq_binop_default bop.bvxor
           | bop.coalesce => simplify_eq_binop_default bop.coalesce
+          | bop.mulx => simplify_eq_binop_default bop.mulx
           | bop.bvapp => simplify_eq_binop_bvapp
           | bop.bvcons => simplify_eq_binop_bvcons
           | bop.update_vector_subrange s l =>
